parse identifiers as global in bedrock2
they used to be parsed as ident, which resulted in only local scope
being used to resolve them. Ideally, we would allow both, but
coq/coq#9755, so we use global instead. Uses of "_"  for holes in
bedrock2 code need to be replaced with "constr:(_)".

bedrock2/src/Examples/swap.v
@@ -4,15 +4,17 @@ Import Syntax BinInt String List.ListNotations.
 Local Open Scope string_scope. Local Open Scope Z_scope. Local Open Scope list_scope.
 Local Existing Instance bedrock2.BasicCSyntax.StringNames_params.
 Local Coercion var (x : string) : Syntax.expr := Syntax.expr.var x.
+Local Definition bedrock_func : Type := funname * (list varname * list varname * cmd).
+Local Coercion name_of_func (f : bedrock_func) := fst f.
 
-Definition swap := let a := "a" in let b := "b" in let t := "t" in
+Definition swap : bedrock_func := let a := "a" in let b := "b" in let t := "t" in
   ("swap", ([a; b], ([]:list varname), bedrock_func_body:(
   t = (load(b)) ;
   store(b, load(a));
   store(a, t)
 ))).
 
-Definition swap_swap := let swap := "swap" in let a := "a" in let b := "b" in
+Definition swap_swap := let a := "a" in let b := "b" in
   ("swap_swap", (("a"::"b"::nil), ([]:list varname), bedrock_func_body:(
   swap(a, b);
   swap(a, b)
