bedrock2/src/NotationsCustomEntry.v
@@ -10,7 +10,7 @@ Notation "bedrock_expr:( e )"   := e   (e custom bedrock_expr,
 Notation "constr:( e )"         := e   (in custom bedrock_expr, e constr,
                                         format "'constr:(' e ')'").
 Notation  "( e )" := e                 (in custom bedrock_expr at level 0).
-Notation "x" := x (in custom bedrock_expr at level 0, x ident).
+Notation "x" := x (in custom bedrock_expr at level 0, x global).
 
 Infix  "<<" := (expr.op slu)  (in custom bedrock_expr at level 3, left associativity). (* DRAFT level *)
 Infix  ">>" := (expr.op sru)  (in custom bedrock_expr at level 3, left associativity). (* DRAFT level *)
@@ -53,7 +53,7 @@ Notation "bedrock_cmd:( c )"   := c   (c custom bedrock_cmd at level 0,
 Notation "constr:( c )"        := c   (in custom bedrock_cmd, c constr,
                                        format "'constr:(' c ')'").
 Notation  "{ c }" := c                 (in custom bedrock_cmd at level 0).
-Notation "x" := x (in custom bedrock_cmd at level 0, x ident).
+Notation "x" := x (in custom bedrock_cmd at level 0, x global).
 
 Declare Custom Entry bedrock_else.
 Notation "bedrock_else:( c )"   := c   (c custom bedrock_else at level 0,
@@ -62,7 +62,7 @@ Notation "constr:( c )"        := c   (in custom bedrock_else, c constr,
                                        format "'constr:(' c ')'").
 Notation  "{ c }" := c                 (in custom bedrock_else at level 0, c custom bedrock_cmd at level 0,
                                        format "{  '/  ' c '/' }").
-Notation "x" := x (in custom bedrock_else at level 0, x ident).
+Notation "x" := x (in custom bedrock_else at level 0, x global).
 
 Notation "'if' e { c1 }" := (cond e c1 skip)
   (in custom bedrock_else at level 0, no associativity, e custom bedrock_expr, c1 custom bedrock_cmd at level 0,
@@ -101,43 +101,43 @@ Notation "bedrock_call_lhs:( e )"   := e   (e custom bedrock_call_lhs,
                                             format "'bedrock_call_lhs:(' e ')'").
 Notation "constr:( e )"         := e   (in custom bedrock_call_lhs, e constr,
                                         format "'constr:(' e ')'").
-Notation "x" := (@cons varname x nil) (in custom bedrock_call_lhs at level 0, x ident).
+Notation "x" := (@cons varname x nil) (in custom bedrock_call_lhs at level 0, x global).
 Notation "x , y , .. , z" := (@cons varname x (@cons varname y .. (@cons varname z (@nil varname)) ..))
-  (in custom bedrock_call_lhs at level 0, x ident, y constr at level 0, z constr at level 0).
+  (in custom bedrock_call_lhs at level 0, x global, y constr at level 0, z constr at level 0).
 
 (* COQBUG(9532) *)
 (* functions of up to 6 arguments *)
-Notation "f ( )" :=  (call nil f nil) (in custom bedrock_cmd at level 0, f ident).
-Notation "f ( x )" :=  (call nil f (@cons expr x nil)) (in custom bedrock_cmd at level 0, f ident, x custom bedrock_expr).
-Notation "f ( x , y )" :=  (call nil f (@cons expr x (@cons expr y nil))) (in custom bedrock_cmd at level 0, f ident, x custom bedrock_expr, y custom bedrock_expr).
-Notation "f ( x , y , z )" :=  (call nil f (@cons expr x (@cons expr y (@cons expr z (@nil expr))))) (in custom bedrock_cmd at level 0, f ident, x custom bedrock_expr, y custom bedrock_expr, z custom bedrock_expr).
-Notation "f ( x , y , z , a )" :=  (call nil f (@cons expr x (@cons expr y (@cons expr z (@cons expr a (@nil expr)))))) (in custom bedrock_cmd at level 0, f ident, x custom bedrock_expr, y custom bedrock_expr, z custom bedrock_expr, a custom bedrock_expr).
-Notation "f ( x , y , z , a , b )" :=  (call nil f (@cons expr x (@cons expr y (@cons expr z (@cons expr a (@cons expr b (@nil expr))))))) (in custom bedrock_cmd at level 0, f ident, x custom bedrock_expr, y custom bedrock_expr, z custom bedrock_expr, a custom bedrock_expr, b custom bedrock_expr).
-Notation "f ( x , y , z , a , b , c )" :=  (call nil f (@cons expr x (@cons expr y (@cons expr z (@cons expr a (@cons expr b (@cons expr c (@nil expr)))))))) (in custom bedrock_cmd at level 0, f ident, x custom bedrock_expr, y custom bedrock_expr, z custom bedrock_expr, a custom bedrock_expr, b custom bedrock_expr, c custom bedrock_expr).
+Notation "f ( )" :=  (call nil f nil) (in custom bedrock_cmd at level 0, f global).
+Notation "f ( x )" :=  (call nil f (@cons expr x nil)) (in custom bedrock_cmd at level 0, f global, x custom bedrock_expr).
+Notation "f ( x , y )" :=  (call nil f (@cons expr x (@cons expr y nil))) (in custom bedrock_cmd at level 0, f global, x custom bedrock_expr, y custom bedrock_expr).
+Notation "f ( x , y , z )" :=  (call nil f (@cons expr x (@cons expr y (@cons expr z (@nil expr))))) (in custom bedrock_cmd at level 0, f global, x custom bedrock_expr, y custom bedrock_expr, z custom bedrock_expr).
+Notation "f ( x , y , z , a )" :=  (call nil f (@cons expr x (@cons expr y (@cons expr z (@cons expr a (@nil expr)))))) (in custom bedrock_cmd at level 0, f global, x custom bedrock_expr, y custom bedrock_expr, z custom bedrock_expr, a custom bedrock_expr).
+Notation "f ( x , y , z , a , b )" :=  (call nil f (@cons expr x (@cons expr y (@cons expr z (@cons expr a (@cons expr b (@nil expr))))))) (in custom bedrock_cmd at level 0, f global, x custom bedrock_expr, y custom bedrock_expr, z custom bedrock_expr, a custom bedrock_expr, b custom bedrock_expr).
+Notation "f ( x , y , z , a , b , c )" :=  (call nil f (@cons expr x (@cons expr y (@cons expr z (@cons expr a (@cons expr b (@cons expr c (@nil expr)))))))) (in custom bedrock_cmd at level 0, f global, x custom bedrock_expr, y custom bedrock_expr, z custom bedrock_expr, a custom bedrock_expr, b custom bedrock_expr, c custom bedrock_expr).
 
-Notation "unpack! lhs = f ( )" :=  (call lhs f nil) (in custom bedrock_cmd at level 0, lhs custom bedrock_call_lhs, f ident).
-Notation "unpack! lhs = f ( x )" :=  (call lhs f (@cons expr x nil)) (in custom bedrock_cmd at level 0, lhs custom bedrock_call_lhs, f ident, x custom bedrock_expr).
-Notation "unpack! lhs = f ( x , y )" :=  (call lhs f (@cons expr x (@cons expr y nil))) (in custom bedrock_cmd at level 0, lhs custom bedrock_call_lhs, f ident, x custom bedrock_expr, y custom bedrock_expr).
-Notation "unpack! lhs = f ( x , y , z )" :=  (call lhs f (@cons expr x (@cons expr y (@cons expr z (@nil expr))))) (in custom bedrock_cmd at level 0, lhs custom bedrock_call_lhs, f ident, x custom bedrock_expr, y custom bedrock_expr, z custom bedrock_expr).
-Notation "unpack! lhs = f ( x , y , z , a )" :=  (call lhs f (@cons expr x (@cons expr y (@cons expr z (@cons expr a (@nil expr)))))) (in custom bedrock_cmd at level 0, lhs custom bedrock_call_lhs, f ident, x custom bedrock_expr, y custom bedrock_expr, z custom bedrock_expr, a custom bedrock_expr).
-Notation "unpack! lhs = f ( x , y , z , a , b )" :=  (call lhs f (@cons expr x (@cons expr y (@cons expr z (@cons expr a (@cons b (@nil expr))))))) (in custom bedrock_cmd at level 0, lhs custom bedrock_call_lhs, f ident, x custom bedrock_expr, y custom bedrock_expr, z custom bedrock_expr, a custom bedrock_expr, b custom bedrock_expr).
-Notation "unpack! lhs = f ( x , y , z , a , b , c )" :=  (call lhs f (@cons expr x (@cons expr y (@cons expr z (@cons expr a (@cons expr b (@cons expr c (@nil expr)))))))) (in custom bedrock_cmd at level 0, lhs custom bedrock_call_lhs, f ident, x custom bedrock_expr, y custom bedrock_expr, z custom bedrock_expr, a custom bedrock_expr, b custom bedrock_expr, c custom bedrock_expr).
+Notation "unpack! lhs = f ( )" :=  (call lhs f nil) (in custom bedrock_cmd at level 0, lhs custom bedrock_call_lhs, f global).
+Notation "unpack! lhs = f ( x )" :=  (call lhs f (@cons expr x nil)) (in custom bedrock_cmd at level 0, lhs custom bedrock_call_lhs, f global, x custom bedrock_expr).
+Notation "unpack! lhs = f ( x , y )" :=  (call lhs f (@cons expr x (@cons expr y nil))) (in custom bedrock_cmd at level 0, lhs custom bedrock_call_lhs, f global, x custom bedrock_expr, y custom bedrock_expr).
+Notation "unpack! lhs = f ( x , y , z )" :=  (call lhs f (@cons expr x (@cons expr y (@cons expr z (@nil expr))))) (in custom bedrock_cmd at level 0, lhs custom bedrock_call_lhs, f global, x custom bedrock_expr, y custom bedrock_expr, z custom bedrock_expr).
+Notation "unpack! lhs = f ( x , y , z , a )" :=  (call lhs f (@cons expr x (@cons expr y (@cons expr z (@cons expr a (@nil expr)))))) (in custom bedrock_cmd at level 0, lhs custom bedrock_call_lhs, f global, x custom bedrock_expr, y custom bedrock_expr, z custom bedrock_expr, a custom bedrock_expr).
+Notation "unpack! lhs = f ( x , y , z , a , b )" :=  (call lhs f (@cons expr x (@cons expr y (@cons expr z (@cons expr a (@cons b (@nil expr))))))) (in custom bedrock_cmd at level 0, lhs custom bedrock_call_lhs, f global, x custom bedrock_expr, y custom bedrock_expr, z custom bedrock_expr, a custom bedrock_expr, b custom bedrock_expr).
+Notation "unpack! lhs = f ( x , y , z , a , b , c )" :=  (call lhs f (@cons expr x (@cons expr y (@cons expr z (@cons expr a (@cons expr b (@cons expr c (@nil expr)))))))) (in custom bedrock_cmd at level 0, lhs custom bedrock_call_lhs, f global, x custom bedrock_expr, y custom bedrock_expr, z custom bedrock_expr, a custom bedrock_expr, b custom bedrock_expr, c custom bedrock_expr).
 
-Notation "output! f ( )" :=  (interact nil f nil) (in custom bedrock_cmd at level 0, f ident).
-Notation "output! f ( x )" :=  (interact nil f (@cons expr x nil)) (in custom bedrock_cmd at level 0, f ident, x custom bedrock_expr).
-Notation "output! f ( x , y )" :=  (interact nil f (@cons expr x (@cons expr y nil))) (in custom bedrock_cmd at level 0, f ident, x custom bedrock_expr, y custom bedrock_expr).
-Notation "output! f ( x , y , z )" :=  (interact nil f (@cons expr x (@cons expr y (@cons expr z (@nil expr))))) (in custom bedrock_cmd at level 0, f ident, x custom bedrock_expr, y custom bedrock_expr, z custom bedrock_expr).
-Notation "output! f ( x , y , z , a )" :=  (interact nil f (@cons expr x (@cons expr y (@cons expr z (@cons expr a (@nil expr)))))) (in custom bedrock_cmd at level 0, f ident, x custom bedrock_expr, y custom bedrock_expr, z custom bedrock_expr, a custom bedrock_expr).
-Notation "output! f ( x , y , z , a , b )" :=  (interact nil f (@cons expr x (@cons expr y (@cons expr z (@cons expr a (@cons expr b (@nil expr))))))) (in custom bedrock_cmd at level 0, f ident, x custom bedrock_expr, y custom bedrock_expr, z custom bedrock_expr, a custom bedrock_expr, b custom bedrock_expr).
-Notation "output! f ( x , y , z , a , b , c )" :=  (interact nil f (@cons expr x (@cons expr y (@cons expr z (@cons expr a (@cons expr b (@cons expr c (@nil expr)))))))) (in custom bedrock_cmd at level 0, f ident, x custom bedrock_expr, y custom bedrock_expr, z custom bedrock_expr, a custom bedrock_expr, b custom bedrock_expr, c custom bedrock_expr).
+Notation "output! f ( )" :=  (interact nil f nil) (in custom bedrock_cmd at level 0, f global).
+Notation "output! f ( x )" :=  (interact nil f (@cons expr x nil)) (in custom bedrock_cmd at level 0, f global, x custom bedrock_expr).
+Notation "output! f ( x , y )" :=  (interact nil f (@cons expr x (@cons expr y nil))) (in custom bedrock_cmd at level 0, f global, x custom bedrock_expr, y custom bedrock_expr).
+Notation "output! f ( x , y , z )" :=  (interact nil f (@cons expr x (@cons expr y (@cons expr z (@nil expr))))) (in custom bedrock_cmd at level 0, f global, x custom bedrock_expr, y custom bedrock_expr, z custom bedrock_expr).
+Notation "output! f ( x , y , z , a )" :=  (interact nil f (@cons expr x (@cons expr y (@cons expr z (@cons expr a (@nil expr)))))) (in custom bedrock_cmd at level 0, f global, x custom bedrock_expr, y custom bedrock_expr, z custom bedrock_expr, a custom bedrock_expr).
+Notation "output! f ( x , y , z , a , b )" :=  (interact nil f (@cons expr x (@cons expr y (@cons expr z (@cons expr a (@cons expr b (@nil expr))))))) (in custom bedrock_cmd at level 0, f global, x custom bedrock_expr, y custom bedrock_expr, z custom bedrock_expr, a custom bedrock_expr, b custom bedrock_expr).
+Notation "output! f ( x , y , z , a , b , c )" :=  (interact nil f (@cons expr x (@cons expr y (@cons expr z (@cons expr a (@cons expr b (@cons expr c (@nil expr)))))))) (in custom bedrock_cmd at level 0, f global, x custom bedrock_expr, y custom bedrock_expr, z custom bedrock_expr, a custom bedrock_expr, b custom bedrock_expr, c custom bedrock_expr).
 
-Notation "io! lhs = f ( )" :=  (interact lhs f nil) (in custom bedrock_cmd at level 0, lhs custom bedrock_call_lhs, f ident).
-Notation "io! lhs = f ( x )" :=  (interact lhs f (@cons expr x nil)) (in custom bedrock_cmd at level 0, lhs custom bedrock_call_lhs, f ident, x custom bedrock_expr).
-Notation "io! lhs = f ( x , y )" :=  (interact lhs f (@cons expr x (@cons expr y nil))) (in custom bedrock_cmd at level 0, lhs custom bedrock_call_lhs, f ident, x custom bedrock_expr, y custom bedrock_expr).
-Notation "io! lhs = f ( x , y , z )" :=  (interact lhs f (@cons expr x (@cons expr y (@cons expr z (@nil expr))))) (in custom bedrock_cmd at level 0, lhs custom bedrock_call_lhs, f ident, x custom bedrock_expr, y custom bedrock_expr, z custom bedrock_expr).
-Notation "io! lhs = f ( x , y , z , a )" :=  (interact lhs f (@cons expr x (@cons expr y (@cons expr z (@cons expr a (@nil expr)))))) (in custom bedrock_cmd at level 0, lhs custom bedrock_call_lhs, f ident, x custom bedrock_expr, y custom bedrock_expr, z custom bedrock_expr, a custom bedrock_expr).
-Notation "io! lhs = f ( x , y , z , a , b )" :=  (interact lhs f (@cons expr x (@cons expr y (@cons expr z (@cons expr a (@cons b (@nil expr))))))) (in custom bedrock_cmd at level 0, lhs custom bedrock_call_lhs, f ident, x custom bedrock_expr, y custom bedrock_expr, z custom bedrock_expr, a custom bedrock_expr, b custom bedrock_expr).
-Notation "io! lhs = f ( x , y , z , a , b , c )" :=  (interact lhs f (@cons expr x (@cons expr y (@cons expr z (@cons expr a (@cons expr b (@cons expr c (@nil expr)))))))) (in custom bedrock_cmd at level 0, lhs custom bedrock_call_lhs, f ident, x custom bedrock_expr, y custom bedrock_expr, z custom bedrock_expr, a custom bedrock_expr, b custom bedrock_expr, c custom bedrock_expr).
+Notation "io! lhs = f ( )" :=  (interact lhs f nil) (in custom bedrock_cmd at level 0, lhs custom bedrock_call_lhs, f global).
+Notation "io! lhs = f ( x )" :=  (interact lhs f (@cons expr x nil)) (in custom bedrock_cmd at level 0, lhs custom bedrock_call_lhs, f global, x custom bedrock_expr).
+Notation "io! lhs = f ( x , y )" :=  (interact lhs f (@cons expr x (@cons expr y nil))) (in custom bedrock_cmd at level 0, lhs custom bedrock_call_lhs, f global, x custom bedrock_expr, y custom bedrock_expr).
+Notation "io! lhs = f ( x , y , z )" :=  (interact lhs f (@cons expr x (@cons expr y (@cons expr z (@nil expr))))) (in custom bedrock_cmd at level 0, lhs custom bedrock_call_lhs, f global, x custom bedrock_expr, y custom bedrock_expr, z custom bedrock_expr).
+Notation "io! lhs = f ( x , y , z , a )" :=  (interact lhs f (@cons expr x (@cons expr y (@cons expr z (@cons expr a (@nil expr)))))) (in custom bedrock_cmd at level 0, lhs custom bedrock_call_lhs, f global, x custom bedrock_expr, y custom bedrock_expr, z custom bedrock_expr, a custom bedrock_expr).
+Notation "io! lhs = f ( x , y , z , a , b )" :=  (interact lhs f (@cons expr x (@cons expr y (@cons expr z (@cons expr a (@cons b (@nil expr))))))) (in custom bedrock_cmd at level 0, lhs custom bedrock_call_lhs, f global, x custom bedrock_expr, y custom bedrock_expr, z custom bedrock_expr, a custom bedrock_expr, b custom bedrock_expr).
+Notation "io! lhs = f ( x , y , z , a , b , c )" :=  (interact lhs f (@cons expr x (@cons expr y (@cons expr z (@cons expr a (@cons expr b (@cons expr c (@nil expr)))))))) (in custom bedrock_cmd at level 0, lhs custom bedrock_call_lhs, f global, x custom bedrock_expr, y custom bedrock_expr, z custom bedrock_expr, a custom bedrock_expr, b custom bedrock_expr, c custom bedrock_expr).
 
 Delimit Scope bedrock_tail with bedrock_tail.
 Notation "bedrock_func_body:( c )"   := (c%bedrock_tail) (c custom bedrock_cmd at level 0,
@@ -161,67 +161,67 @@ Module test.
   
   Goal True.
   assert (p : parameters) by admit.
-  epose (fun x => bedrock_cmd:( store1(1<<(1+1+1), 1+1) ; if 1 { store1(1,1) } ; _ = (1) )).
-  epose (fun a => bedrock_cmd:( if 1 { _ = (1);  _ = (a) } )).
+  epose (fun x => bedrock_cmd:( store1(1<<(1+1+1), 1+1) ; if 1 { store1(1,1) } ; constr:(_) = (1) )).
+  epose (fun a => bedrock_cmd:( if 1 { constr:(_) = (1);  constr:(_) = (a) } )).
   epose (fun a => bedrock_cmd:( a (1+1 , 1+1,1, 1 ) )).
   epose (fun a => bedrock_cmd:( a (1+1 , 1+1,1, 1 ,1 ) )).
   epose (fun a => bedrock_cmd:( a (1+1 , 1+1,1, 1,1,1 ) )).
   epose (fun (a b c d:varname) (f:funname) => bedrock_cmd:( unpack! a,b,c,d = f ( 1 + 1 , 1 + 1 ) )).
   epose (fun (a b:varname) (f:funname) => bedrock_cmd:( unpack! a = f ( 1 + 1 , 1 + 1 ) ; a = (1) )).
-  epose (fun (a b:varname) (f:funname) => bedrock_cmd:( if _ { _ } else if _ { _ } )).
+  epose (fun (a b:varname) (f:funname) => bedrock_cmd:( if constr:(_) { constr:(_) } else if constr:(_) { constr:(_) } )).
 
   epose (bedrock_cmd:(
-      if _ { _ }
-      else if _ { _ }
-      else if _ { _ }
-      else if _ { _ };
-      _)).
+      if constr:(_) { constr:(_) }
+      else if constr:(_) { constr:(_) }
+      else if constr:(_) { constr:(_) }
+      else if constr:(_) { constr:(_) };
+      constr:(_))).
 
-  epose bedrock_func_body:( require _ else { _ } ; _ ).
-  epose bedrock_func_body:( require _ ; _ ).
+  epose bedrock_func_body:( require constr:(_) else { constr:(_) } ; constr:(_) ).
+  epose bedrock_func_body:( require constr:(_) ; constr:(_) ).
 
   epose bedrock_func_body:(
       if (1<<(1+1)*(1+1) ^ (1+1+1)) {
-          require (1 ^ 1 == 1) else { _ }; _
+          require (1 ^ 1 == 1) else { constr:(_) }; constr:(_)
       }).
 
   epose bedrock_func_body:(
       if (1<<(1+1)*(1+1) ^ (1+1+1)) {
-             _ } else {
-          require (1 ^ 1) else { _ }; _
+             constr:(_) } else {
+          require (1 ^ 1) else { constr:(_) }; constr:(_)
       }).
 
   epose bedrock_func_body:(
    require (1 ^ 1) else {
-       require (1 ^ 1) else { _ };
-       _
+       require (1 ^ 1) else { constr:(_) };
+       constr:(_)
    };
-    _
+    constr:(_)
   ).
 
   assert_fails (epose bedrock_func_body:(
-    if (1) { require (1 ^ 1) else { _ }; _  } ;
-    { _ = (_)}
+    if (1) { require (1 ^ 1) else { constr:(_) }; constr:(_)  } ;
+    { constr:(_) = (constr:(_))}
   )).
 
   assert_fails (epose bedrock_func_body:(
-    if (1) { require (1 ^ 1) else { _ }; _  }
-    else { _ };
-    _ = (_)
+    if (1) { require (1 ^ 1) else { constr:(_) }; constr:(_)  }
+    else { constr:(_) };
+    constr:(_) = (constr:(_))
   )).
 
   assert_fails (epose bedrock_func_body:(
-    if (1) { _  } else { require (1 ^ 1) else { _ }; _ };
-    { _ = (_)}
+    if (1) { constr:(_)  } else { require (1 ^ 1) else { constr:(_) }; constr:(_) };
+    { constr:(_) = (constr:(_))}
   )).
   
   assert_fails (epose bedrock_func_body:(
-    while (1) { require (1 ^ 1) else { _ }; _ };
-    { _ = (_)}
+    while (1) { require (1 ^ 1) else { constr:(_) }; constr:(_) };
+    { constr:(_) = (constr:(_))}
   )).
 
   assert_fails (epose bedrock_func_body:(
-    while (1) { require (1 ^ 1) else { _ }; _ = (_) }
+    while (1) { require (1 ^ 1) else { constr:(_) }; constr:(_) = (constr:(_)) }
   )).
 
   let lhs := open_constr:( bedrock_func_body:(
@@ -245,15 +245,15 @@ Module test.
   assert (lhs = rhs) by exact eq_refl.
 
   epose (fun W a b e x y f read write => bedrock_func_body:(
-    require (load(1) ^ constr:(expr.literal 231321) ) else { _ };
-    require (1 ^ load4(1+1+1+load(1))) else { _ };
+    require (load(1) ^ constr:(expr.literal 231321) ) else { constr:(_) };
+    require (1 ^ load4(1+1+1+load(1))) else { constr:(_) };
     { a = (1+1 == 1) } ;
-    require (1 ^ 1) else { _ };
+    require (1 ^ 1) else { constr:(_) };
     store1(e, load2(1)+load4(1)+load1(load(1))) ;
     store2(e, 1+1+1);
     store4(e, 1+1+1) ;
     store(e, load(load(load(1))));
-    require (1 ^ 1) else { _ };
+    require (1 ^ 1) else { constr:(_) };
     if (W+1<<(1+1)*(1+1) ^ (1+1+1)) {
       a = (constr:(expr.var x))
     } else {
